Backport proofs for constant_time_ops.rs

libcrux-ml-kem/src/constant_time_ops.rs
@@ -71,9 +71,7 @@ fn is_non_zero(value: u8) -> u8 {
 
 /// Return 1 if the bytes of `lhs` and `rhs` do not exactly
 /// match and 0 otherwise.
-#[cfg_attr(hax, hax_lib::requires(
-    lhs.len() == rhs.len()
-))]
+#[hax_lib::requires(lhs.len() == rhs.len())]
 #[hax_lib::ensures(|result| fstar!("Hax_lib.implies ($lhs =. $rhs <: bool)
     (fun temp_0_ ->
         let _:Prims.unit = temp_0_ in
@@ -126,25 +124,72 @@ fn compare(lhs: &[u8], rhs: &[u8]) -> u8 {
 
 /// If `selector` is not zero, return the bytes in `rhs`; return the bytes in
 /// `lhs` otherwise.
-#[cfg_attr(hax, hax_lib::requires(
+#[hax_lib::requires(
     lhs.len() == rhs.len() &&
     lhs.len() == SHARED_SECRET_SIZE
-))]
+)]
+#[hax_lib::ensures(|result| fstar!("Hax_lib.implies ($selector =. 0uy <: bool)
+            (fun _ -> $result =. $lhs <: bool) &&
+        Hax_lib.implies ($selector <>. 0uy <: bool) (fun _ -> $result =. $rhs <: bool)"))]
+#[hax_lib::fstar::options("--ifuel 0 --z3rlimit 50")]
 fn select_ct(lhs: &[u8], rhs: &[u8], selector: u8) -> [u8; SHARED_SECRET_SIZE] {
     let mask = is_non_zero(selector).wrapping_sub(1);
+    hax_lib::fstar!("assert (if $selector = 0uy then $mask = ones else $mask = zero);
+        lognot_lemma $mask;
+        assert (if $selector = 0uy then ~.$mask = zero else ~.$mask = ones)");
     let mut out = [0u8; SHARED_SECRET_SIZE];
 
     for i in 0..SHARED_SECRET_SIZE {
-        out[i] = (lhs[i] & mask) | (rhs[i] & !mask);
+        hax_lib::loop_invariant!(|i: usize| { fstar!("v $i <= v $SHARED_SECRET_SIZE /\\
+            (forall j. j < v $i ==> (if ($selector =. 0uy) then Seq.index $out j == Seq.index $lhs j else Seq.index $out j == Seq.index $rhs j)) /\\
+            (forall j. j >= v $i ==> Seq.index $out j == 0uy)") });
+        hax_lib::fstar!("assert ((${out}.[ $i ] <: u8) = 0uy)");
+        let outi = (lhs[i] & mask) | (rhs[i] & !mask);
+        hax_lib::fstar!("if ($selector = 0uy) then (
+            logand_lemma (${lhs}.[ $i ] <: u8) $mask;
+            assert (((${lhs}.[ $i ] <: u8) &. $mask <: u8) == (${lhs}.[ $i ] <: u8));
+            logand_lemma (${rhs}.[ $i ] <: u8) (~.$mask);
+            assert (((${rhs}.[ $i ] <: u8) &. (~.$mask <: u8) <: u8) == zero);
+            logor_lemma ((${lhs}.[ $i ] <: u8) &. $mask <: u8) ((${rhs}.[ $i ] <: u8) &. (~.$mask <: u8) <: u8);
+            assert ((((${lhs}.[ $i ] <: u8) &. $mask <: u8) |. ((${rhs}.[ $i ] <: u8) &. (~.$mask <: u8) <: u8) <: u8) == (${lhs}.[ $i ] <: u8));
+            logor_lemma (${out}.[ $i ] <: u8) (${lhs}.[ $i ] <: u8);
+            assert (((${out}.[ $i ] <: u8) |. (((${lhs}.[ $i ] <: u8) &. $mask <: u8) |. ((${rhs}.[ $i ] <: u8) &. (~.$mask <: u8) <: u8) <: u8) <: u8) == (${lhs}.[ $i ] <: u8));
+            assert ($outi = (${lhs}.[ $i ] <: u8))
+          )
+          else (
+            logand_lemma (${lhs}.[ $i ] <: u8) $mask;
+            assert (((${lhs}.[ $i ] <: u8) &. $mask <: u8) == zero);
+            logand_lemma (${rhs}.[ $i ] <: u8) (~.$mask);
+            assert (((${rhs}.[ $i ] <: u8) &. (~.$mask <: u8) <: u8) == (${rhs}.[ $i ] <: u8));
+            logor_lemma (${rhs}.[ $i ] <: u8) zero;
+            assert ((logor zero (${rhs}.[ $i ] <: u8)) == (${rhs}.[ $i ] <: u8));
+            assert ((((${lhs}.[ $i ] <: u8) &. $mask <: u8) |. ((${rhs}.[ $i ] <: u8) &. (~.$mask <: u8) <: u8)) == (${rhs}.[ $i ] <: u8));
+            logor_lemma (${out}.[ $i ] <: u8) (${rhs}.[ $i ] <: u8);
+            assert (((${out}.[ $i ] <: u8) |. (((${lhs}.[ $i ] <: u8) &. $mask <: u8) |. ((${rhs}.[ $i ] <: u8) &. (~.$mask <: u8) <: u8) <: u8) <: u8) == (${rhs}.[ $i ] <: u8));
+            assert ($outi = (${rhs}.[ $i ] <: u8))
+          )");
+        out[i] = outi;
     }
 
+    hax_lib::fstar!("if ($selector =. 0uy) then (
+            eq_intro $out $lhs
+        )
+        else (
+            eq_intro $out $rhs
+        )");
     out
 }
 
 #[inline(never)] // Don't inline this to avoid that the compiler optimizes this out.
-#[cfg_attr(hax, hax_lib::requires(
-    lhs.len() == rhs.len()
-))]
+#[hax_lib::requires(lhs.len() == rhs.len())]
+#[hax_lib::ensures(|result| fstar!("Hax_lib.implies ($lhs =. $rhs <: bool)
+    (fun temp_0_ ->
+        let _:Prims.unit = temp_0_ in
+        $result =. 0uy <: bool) &&
+    Hax_lib.implies ($lhs <>. $rhs <: bool)
+    (fun temp_0_ ->
+        let _:Prims.unit = temp_0_ in
+        $result =. 1uy <: bool)"))]
 pub(crate) fn compare_ciphertexts_in_constant_time(lhs: &[u8], rhs: &[u8]) -> u8 {
     #[cfg(eurydice)]
     return compare(lhs, rhs);
@@ -154,10 +199,13 @@ pub(crate) fn compare_ciphertexts_in_constant_time(lhs: &[u8], rhs: &[u8]) -> u8
 }
 
 #[inline(never)] // Don't inline this to avoid that the compiler optimizes this out.
-#[cfg_attr(hax, hax_lib::requires(
+#[hax_lib::requires(
     lhs.len() == rhs.len() &&
     lhs.len() == SHARED_SECRET_SIZE
-))]
+)]
+#[hax_lib::ensures(|result| fstar!("Hax_lib.implies ($selector =. 0uy <: bool)
+            (fun _ -> $result =. $lhs <: bool) &&
+        Hax_lib.implies ($selector <>. 0uy <: bool) (fun _ -> $result =. $rhs <: bool)"))]
 pub(crate) fn select_shared_secret_in_constant_time(
     lhs: &[u8],
     rhs: &[u8],
@@ -170,11 +218,15 @@ pub(crate) fn select_shared_secret_in_constant_time(
     core::hint::black_box(select_ct(lhs, rhs, selector))
 }
 
-#[cfg_attr(hax, hax_lib::requires(
+#[hax_lib::requires(
     lhs_c.len() == rhs_c.len() &&
     lhs_s.len() == rhs_s.len() &&
     lhs_s.len() == SHARED_SECRET_SIZE
-))]
+)]
+#[hax_lib::ensures(|result| fstar!("let selector = if $lhs_c =. $rhs_c then 0uy else 1uy in
+    Hax_lib.implies (selector =. 0uy <: bool)
+        (fun _ -> $result =. $lhs_s <: bool) &&
+    Hax_lib.implies (selector <>. 0uy <: bool) (fun _ -> $result =. $rhs_s <: bool)"))]
 pub(crate) fn compare_ciphertexts_select_shared_secret_in_constant_time(
     lhs_c: &[u8],
     rhs_c: &[u8],
